\documentclass[12pt]{ctexart}
\usepackage{amsmath}
\usepackage{amssymb}
\usepackage{amsthm}
\usepackage{color}
\usepackage{graphicx}
\usepackage{geometry}
\usepackage{hyperref}
\usepackage{marginnote}
\usepackage{mathrsfs}
\usepackage{syntonly}
\usepackage{textcomp}
\usepackage{ulem}
\usepackage{verbatim}
%\syntaxonly
%\geometry{a5paper}
\hyphenation{}
\normalem
\hypersetup{
    colorlinks,
    linkcolor=blue,
    filecolor=pink,
    urlcolor=cyan,
    citecolor=red,
}
\def\b{\boldsymbol}
\def\d{\mathrm{d}}
\def\p{\partial}
\def\ph{\phantom}
\def\t{\tilde}
\def\Ra{\Rightarrow}
\newcommand{\tabincell}[2]{\begin{tabular}{@{}#1@{}}#2\end{tabular}}
\DeclareMathOperator{\sgn}{sgn}
\DeclareMathOperator{\atanxy}{atan2}
\theoremstyle{definition}
\newtheorem{definition}{定义}
\newtheorem{proposition}{命题}
\title{}
\author{}
\begin{document}
\begin{equation}
    \p^a\p_a A_b=-\mu J_b
\end{equation}
\end{document}

\begin{equation}
    \p^a(\varepsilon A_a)=0
\end{equation}
\begin{equation}
    \p^i[\varepsilon(\p_i A_0-\p_0 A_i)]+J_0=0
\end{equation}
\begin{equation}
    -\p^0[\varepsilon(\p_0 A_j-\p_j A_0)]+\p^i[\varepsilon(\p_i A_j-\p_j A_i)]+J_j=0
\end{equation}
\begin{equation}
    -\p^0(\varepsilon A_0)+\p^i(\varepsilon A_i)=0
\end{equation}
\begin{align}
    \p^i[\varepsilon(\p_i A_0-\p_0 A_i)]+J_0
    &=\p^i(\varepsilon\p_i A_0)-\p_0\p^i(\varepsilon A_i)+J_0\\
    &=\p^i(\varepsilon\p_i A_0)-\p^0(\varepsilon\p_0 A_0)+J_0
\end{align}
\begin{align}
    -\p^0[\varepsilon(\p_0 A_j-\p_j A_0)]+\p^i[\varepsilon(\p_i A_j-\p_j A_i)]+J_j
    &=-\varepsilon\p^0\p_0 A_j+\varepsilon\p^0\p_j A_0+\p^i(\varepsilon\p_i A_j)-\p^i(\varepsilon\p_j A_i)+J_j
\end{align}
\begin{equation}
    -\varepsilon\p^0A_0+(\p^i\varepsilon)A_i+\varepsilon\p^iA_i=0
\end{equation}
\begin{equation}
    -(\p_j\varepsilon)(\p^0A_0)-\varepsilon \p_j\p^0A_0+(\p_j\p^i\varepsilon)A_i+(\p^i\varepsilon)(\p_jA_i)+(\p_j\varepsilon)(\p^iA_i)+\varepsilon\p_j\p^iA_i=0
\end{equation}
\begin{equation}
    \varepsilon\p^0\p_j A_0-\p^i(\varepsilon\p_j A_i)=\varepsilon\p^0\p_j A_0-(\p^i\varepsilon)(\p_j A_i)-\varepsilon\p^i\p_j A_i
\end{equation}
\begin{equation}
    \vec{\nabla}\cdot[\varepsilon(-\vec{\nabla}\varphi-\frac{\p}{\p t}\vec{A})]-\rho=0
\end{equation}
\begin{equation}
    -\frac{\p}{\p t}[\varepsilon(\frac{\p}{\p t}\vec{A}+\vec{\nabla}\varphi)]+\vec{\nabla}\cdot[\varepsilon(-\vec{\nabla}\times\vec{A})]+\vec{j}=0
\end{equation}
\begin{equation}
    \frac{\p }{\p t}(\varepsilon\varphi)+\vec{\nabla}\cdot(\varepsilon\vec{A})=0
\end{equation}
\begin{equation}
    \varphi=\frac{\mu}{4\pi}\int\frac{\rho(t-\left\lvert\vec{r}-\vec{r}'\right\rvert)}{\left\lvert\vec{r}-\vec{r}'\right\rvert}\d V'
\end{equation}
\begin{equation}
    \vec{A}=\frac{\mu^{3/2}}{4\pi}\int\frac{\vec{j}(t-\left\lvert\vec{r}-\vec{r}'\right\rvert)}{\mu^{1/2}\left\lvert\vec{r}-\vec{r}'\right\rvert}\d V'
\end{equation}
\begin{equation}
    \p^a[\varepsilon(\p_a A_b-\p_b A_a)]+J_b=0
\end{equation}
\begin{equation}
    \p^a(\varepsilon\p_a A_b)-\p^a(\varepsilon\p_b A_a)+J_b=0
\end{equation}
\begin{equation}
    \p^a[\varepsilon\p_b(A_a+\p_a\chi)]=0
\end{equation}
\begin{equation}
    (\p^a\varepsilon)\p_b A_a+\varepsilon\p^a\p_b A_a+(\p^a\varepsilon)\p_b\p_a\chi+\varepsilon\p^a\p_b\p_a\chi=0
\end{equation}
\begin{equation}
    \varepsilon\p^a[\varepsilon(\p_a A_b-\p_b A_a)]+\varepsilon J_b=0
\end{equation}
\begin{equation}
    \frac{\p}{\p r}=\frac{\p}{\p x}\frac{\p x}{\p r}+\frac{\p}{\p y}\frac{\p y}{\p r}+\frac{\p}{\p z}\frac{\p z}{\p r}=\frac{\p}{\p x}\sin\theta\cos\phi+\frac{\p}{\p y}\sin\theta\sin\phi+\frac{\p}{\p z}\cos\theta
\end{equation}
\begin{equation}
    \frac{\p}{\p \theta}=\frac{\p}{\p x}\frac{\p x}{\p \theta}+\frac{\p}{\p y}\frac{\p y}{\p \theta}+\frac{\p}{\p z}\frac{\p z}{\p \theta}=\frac{\p}{\p x}r\cos\theta\cos\phi+\frac{\p}{\p y}r\cos\theta\sin\phi-\frac{\p}{\p z}r\sin\theta
\end{equation}
\begin{equation}
    \frac{\p}{\p \phi}=\frac{\p}{\p x}\frac{\p x}{\p \phi}+\frac{\p}{\p y}\frac{\p y}{\p \phi}+\frac{\p}{\p z}\frac{\p z}{\p \phi}=-\frac{\p}{\p x}r\sin\theta\sin\phi+\frac{\p}{\p y}r\sin\theta\cos\phi
\end{equation}
\begin{equation}
    t=\varepsilon t',\frac{\p}{\p t'}=\varepsilon\frac{\p}{\p t}
\end{equation}
\begin{align}
    \frac{\p}{\p r'}&=\frac{\p}{\p x'}\frac{x'}{\sqrt{x'^2+y'^2+z'^2}}+\frac{\p}{\p y'}\frac{y'}{\sqrt{x'^2+y'^2+z'^2}}+\frac{\p}{\p z'}\frac{z'}{\sqrt{x'^2+y'^2+z'^2}}\\
    &=\varepsilon(\frac{\p}{\p x}\frac{x}{\sqrt{x^2+y^2+z^2}}+\frac{\p}{\p y}\frac{y}{\sqrt{x^2+y^2+z^2}}+\frac{\p}{\p z}\frac{z}{\sqrt{x^2+y^2+z^2}})\\
    &=\varepsilon\frac{\p}{\p r}
\end{align}
\begin{align}
    \frac{\p}{\p \theta'}&=\frac{\p}{\p x'}z'\frac{x'}{\sqrt{x'^2+y'^2}}+\frac{\p}{\p y'}z'\frac{y'}{\sqrt{x'^2+y'^2}}-\frac{\p}{\p z'}\sqrt{x'^2+y'^2}\\
    &=\frac{\p}{\p x}z\frac{x}{\sqrt{x^2+y^2}}+\frac{\p}{\p y}z\frac{y}{\sqrt{x^2+y^2}}-\frac{\p}{\p z}\sqrt{x^2+y^2}\\
    &=\frac{\p}{\p \theta'}
\end{align}
\begin{align}
    \frac{\p}{\p \phi'}&=-\frac{\p}{\p x'}y'+\frac{\p}{\p y'}x'\\
    &=-\frac{\p}{\p x}y+\frac{\p}{\p y}x\\
    &=\frac{\p}{\p \phi}
\end{align}
\begin{equation}
    \frac{\p}{\p x'}\sin\theta'\cos\phi'+\frac{\p}{\p y'}\sin\theta'\sin\phi'+\frac{\p}{\p z'}\cos\theta'=\varepsilon(\frac{\p}{\p x}\sin\theta\cos\phi+\frac{\p}{\p y}\sin\theta\sin\phi+\frac{\p}{\p z}\cos\theta)
\end{equation}
\begin{equation}
    \frac{\p}{\p x'}r'\cos\theta'\cos\phi'+\frac{\p}{\p y'}r'\cos\theta'\sin\phi'-\frac{\p}{\p z'}r'\sin\theta'=\frac{\p}{\p x}r\cos\theta\cos\phi+\frac{\p}{\p y}r\cos\theta\sin\phi-\frac{\p}{\p z}r\sin\theta
\end{equation}
\begin{equation}
    -\frac{\p}{\p x'}r'\sin\theta'\sin\phi'+\frac{\p}{\p y'}r'\sin\theta'\cos\phi'=-\frac{\p}{\p x}r\sin\theta\sin\phi+\frac{\p}{\p y}r\sin\theta\cos\phi
\end{equation}
\begin{equation}
    \t{t}=\frac{1}{\varepsilon}t,\quad\t{x}=\frac{1}{\varepsilon}x,\quad\t{y}=\frac{1}{\varepsilon}y,\quad\t{z}=\int\frac{1}{\varepsilon}\d z
\end{equation}
\begin{equation}
    \t{\p}^a[(\t{\p}_a A_b-\t{\p}_b A_a)]+\varepsilon J_b=0
\end{equation}
\begin{equation}
    \t{\p}^a\t{\p}_a A_b=-\varepsilon J_b
\end{equation}
\begin{equation}
    A_a=C_ae^{i\omega(\frac{1}{\varepsilon}t-\int\frac{1}{\varepsilon}\d z)}
\end{equation}
\begin{equation}
    A_a=\frac{1}{4\pi}\int\frac{\varepsilon(\t{t}-\t{r},\t{\vec{r}})J_a(\t{t}-\t{r},\t{\vec{r}})}{\t{r}}\d\t{V}
\end{equation}
\begin{equation}
    \p_a v_b=(\d \t{x}^\mu)_a(\d \t{x}^\nu)_b(\t{\p}_\mu\t{v}_\nu-\t{\Gamma}^\sigma_{\ph{\sigma}\mu\nu}\t{v}_\sigma)
\end{equation}
\begin{equation}
    \t{\eta}_{\mu\nu}=\begin{bmatrix}
        -1&0&0&0\\
        0&1&0&0\\
        0&0&r^2&0\\
        0&0&0&r^2\sin^2\theta\\
    \end{bmatrix}
\end{equation}
\begin{equation}
    \t{\Gamma}^0_{\ph{0}\mu\nu}=\begin{bmatrix}
        0&0&0&0\\
        0&0&0&0\\
        0&0&0&0\\
        0&0&0&0\\
    \end{bmatrix}
\end{equation}
\begin{equation}
    \t{\Gamma}^1_{\ph{1}\mu\nu}=\begin{bmatrix}
        0&0&0&0\\
        0&0&0&0\\
        0&0&-r&0\\
        0&0&0&-r\sin^2\theta\\
    \end{bmatrix}
\end{equation}
\begin{equation}
    \t{\Gamma}^2_{\ph{2}\mu\nu}=\begin{bmatrix}
        0&0&0&0\\
        0&0&1/r&0\\
        0&1/r&0&0\\
        0&0&0&-\sin\theta\cos\theta\\
    \end{bmatrix}
\end{equation}
\begin{equation}
    \t{\Gamma}^2_{\ph{2}\mu\nu}=\begin{bmatrix}
        0&0&0&0\\
        0&0&0&1/r\\
        0&0&0&\cos\theta/\sin\theta\\
        0&1/r&\cos\theta/\sin\theta&0\\
    \end{bmatrix}
\end{equation}
\begin{align}
    \p_a v_b&=(\d x^\mu)_a(\d x^\nu)_b\p_\mu v_\nu\\
    &=\frac{\p x^\mu}{\p \t{x}^{\t{\mu}}}(\d \t{x}^{\t{\mu}})_a\frac{\p x^\nu}{\p \t{x}^{\t{\nu}}}(\d \t{x}^{\t{\nu}})_b\frac{\p \t{x}^{\t{\t{\mu}}}}{\p x^\mu}\t{\p}_{\t{\t{\mu}}}(\frac{\p \t{x}^{\t{\t{\nu}}}}{\p x^\nu}\t{v}_{\t{\t{\nu}}})\\
    &=(\d \t{x}^{\t{\mu}})_a(\d \t{x}^{\t{\nu}})_b\frac{\p x^\nu}{\p \t{x}^{\t{\nu}}}\t{\p}_{\t{\mu}}(\frac{\p \t{x}^{\t{\t{\nu}}}}{\p x^\nu}\t{v}_{\t{\t{\nu}}})
\end{align}
\begin{equation}
    \begin{bmatrix}
        \p_r\\\p_\theta\\\p_\phi
    \end{bmatrix}
    \left(\begin{bmatrix}
        \sin\theta\cos\phi&-\sin\theta\sin\phi/r&\cos\theta\cos\phi/r\\
        \sin\theta\sin\phi&\sin\theta\cos\phi/r&\cos\theta\sin\phi/r\\
        \cos\theta&0&-\sin\theta/r\\
    \end{bmatrix}
    \begin{bmatrix}
        v_r\\v_\theta\\v_\phi
    \end{bmatrix}\right)^\text{T}
\end{equation}
\begin{align}
    \p_a v_b&=(\d x^\mu)_a(\d x^\nu)_b\p_\mu v_\nu\\
    &=\frac{\p x^\mu}{\p \t{x}^{\t{\mu}}}(\d \t{x}^{\t{\mu}})_a\frac{\p x^\nu}{\p \t{x}^{\t{\nu}}}(\d \t{x}^{\t{\nu}})_b\frac{\p \t{x}^{\t{\t{\mu}}}}{\p x^\mu}\t{\p}_{\t{\t{\mu}}}(\frac{\p \t{x}^{\t{\t{\nu}}}}{\p x^\nu}\t{v}_{\t{\t{\nu}}})\\
    &=(\d \t{x}^{\t{\mu}})_a(\d \t{x}^{\t{\nu}})_b\frac{\p x^\nu}{\p \t{x}^{\t{\nu}}}\t{\p}_{\t{\mu}}(\frac{\p \t{x}^{\t{\t{\nu}}}}{\p x^\nu}\t{v}_{\t{\t{\nu}}})
\end{align}
\begin{equation}
    -\frac{\p}{\p t}[\varepsilon(\frac{\p}{\p t} A_\lambda-\p_\lambda A_0)]+\vec{\nabla}\cdot[\varepsilon(\vec{\nabla} A_\lambda-\p_\lambda A_i)]+J_\lambda=0
\end{equation}
