\chapter{电磁引力}

\cite{Maartens2008}. 

\section{时空张量转化为空间张量}

\begin{equation}
    h_{ab}:=g_{ab}+Z_a Z_b.
\end{equation}
\begin{equation}
    V_{\langle a\rangle}:=h_a^{\ph{a}b}V_{b}.
\end{equation}
\begin{equation}
    T_{\langle ab\rangle}:=h_{(a}^{\ph{(a}c}h_{b)}^{\ph{b)}d}T_{cd}-\frac{1}{3}h_{cd}T^{cd}h_{ab}.
\end{equation}
\begin{equation}
    \varepsilon_{abc}:=\varepsilon_{abcd}Z^d.
\end{equation}
\begin{equation}
    \varepsilon_{0123}:=-\sqrt{\left\lvert g\right\rvert }
\end{equation}
\begin{equation}
    T_a:=\frac{1}{2}\varepsilon_{abc}T^{[bc]}.
\end{equation}
\begin{equation}
    [U,V]_a:=\varepsilon_{abc}U^bV^c.
\end{equation}
\begin{equation}
    [S,T]_a:=\varepsilon_{abc}S^b_{\ph{b}d}T^{cd}.
\end{equation}
\begin{equation}
    \text{D}_tT^{a\dots}_{\ph{a\dots}b\dots}:=Z^c\nabla_c T^{a\dots}_{\ph{a\dots}b\dots}.
\end{equation}
\begin{equation}
    {}^3\nabla_a T^{b\dots}_{\ph{b\dots}c\dots}:=h_a^{\ph{a}p}h^b_{\ph{b}q}\dots h_c^{\ph{c}r}\dots\nabla_p T^{q\dots}_{\ph{q\dots}r\dots}.
\end{equation}
\begin{equation}
    (\text{div}\,V):={}^3\nabla^aV_a.
\end{equation}
\begin{equation}
    (\text{curl}\,V)_a:=\varepsilon_{abc}{}^3\nabla^bV^c.
\end{equation}
\begin{equation}
    (\text{div}\,T)_a:={}^3\nabla^bT_{ab}.
\end{equation}
\begin{equation}
    (\text{curl}\,T)_{ab}:=\varepsilon_{cd(a}{}^3\nabla^cT_{b)}^{\ph{b)}d}.
\end{equation}

\section{电磁空间矢量}

\begin{equation}
    E_a:=F_{ab}Z^b.
\end{equation}
\begin{equation}
    B_a:={}^*\!F_{ab}Z^b.
\end{equation}
\begin{equation}
    (\text{div}\,E)=\dots.
\end{equation}
\begin{equation}
    (\text{div}\,B)=\dots.
\end{equation}
\begin{equation}
    \text{D}_t E_{\langle a\rangle}-(\text{curl}\,E)_a=\dots.
\end{equation}
\begin{equation}
    \text{D}_t B_{\langle a\rangle}+(\text{curl}\,B)_a=\dots.
\end{equation}

\section{引力空间张量}

\begin{equation}
    E_{ab}:=C_{abcd}Z^cZ^d.
\end{equation}
\begin{equation}
    B_{ab}:={}^*\!C_{abcd}Z^cZ^d.
\end{equation}
\begin{equation}
    (\text{div}\,E)_a=\dots.
\end{equation}
\begin{equation}
    (\text{div}\,B)_a=\dots.
\end{equation}
\begin{equation}
    \text{D}_t E_{\langle ab\rangle}-(\text{curl}\,E)_{ab}=\dots.
\end{equation}
\begin{equation}
    \text{D}_t B_{\langle ab\rangle}+(\text{curl}\,B)_{ab}=\dots.
\end{equation}
