\chapter{宇宙学效应}

\cite{Maggiore2014},
\begin{equation}
    \frac{\d\eta}{\d(ct)}=\frac{1}{a},
\end{equation}
\begin{equation}
    \d s^2=-\d(ct)^2+a^2[\frac{\d r^2}{1-kr^2}+r^2(\d\theta^2+\sin^2\theta\d\phi^2)],
\end{equation}
\begin{equation}
    \d s^2=a^2[-\d\eta^2+\frac{\d r^2}{1-kr^2}+r^2(\d\theta^2+\sin^2\theta\d\phi^2)].
\end{equation}
$\square\Phi=0$, $\Phi:=f/r$, $f:=g/a$,
\begin{equation}
    \p_r^2g+(\p_\eta^2a/a)g-\p_\eta^2g=0,
\end{equation}
$\p_\eta^2a/a\sim\eta^2$, $\omega^2\gg1/\eta^2$,
\begin{equation}
    g\simeq e^{i\omega(\eta-r)}.
\end{equation}
