\chapter{引力波}

\section{Linearized Gravity}

\cite{Wald1984}. 流形$\mathbb{R}^{4}$. 任意坐标系$\{x^{\mu}\}$, $g_{\mu\nu}=\eta_{\mu\nu}+h_{\mu\nu}=\eta_{\mu\nu}+\gamma_{\mu\nu}s+\text{O}(s^2)$, 得
\begin{equation}
    R_{\mu\nu\lambda\sigma}=\p_\sigma\p_{[\mu}h_{\lambda]\nu}-\p_\nu\p_{[\mu}h_{\lambda]\sigma}+\text{O}(s^2).
\end{equation}
$\bar{h}_{\mu\nu}:=h_{\mu\nu}-\frac{1}{2}\eta_{\mu\nu}\eta^{\lambda\sigma}h_{\lambda\sigma}=h_{\mu\nu}-\frac{1}{2}\eta_{\mu\nu}h$.
\begin{equation}
    -\frac{1}{2} \partial^{\lambda} \partial_{\lambda} \bar{h}_{\mu \nu}+\partial^{\lambda} \partial_{(\mu} \bar{h}_{\nu) \lambda}-\frac{1}{2} \eta_{\mu \nu} \partial^{\lambda} \partial^{\sigma} \bar{h}_{\lambda \sigma}+\text{O}(s^2)=8 \pi T_{\mu \nu}.
\end{equation}
存在$\{x^{\mu}\}$, 使得$\p^{\nu}\bar{h}_{\mu\nu}+\text{O}(s^2)=0$ (Lorentz gauge). 
令$\{x^{\mu}\}$满足$\p^{\nu}\bar{h}_{\mu\nu}+\text{O}(s^2)=0$, 则
\begin{equation}
    \p^{\lambda}\p_{\lambda}\bar{h}_{\mu\nu}+\text{O}(s^2)=-16\pi T_{\mu \nu}.\label{lin_gravity}
\end{equation}
略去$\text{O}(s^2)$条件: $h_{\mu\nu}$, $\p_\lambda h_{\mu\nu}$\dots{}小.

\section{Radiation Gauge}

\cite{Wald1984}. 存在$\{x^{\mu}\}$, 使得``无源处'' $h+\text{O}(s^2)=0$ (TT gauge \cite{Wang2020})且$h_{0\mu}+\text{O}(s^2)=0$. 

\section{Quadrupole Approximation}

\cite{Wald1984}. 下略$\text{O}(s^2)$. 由\eqref{lin_gravity}得
\begin{equation}
    \bar{h}_{\mu\nu}(t,\vec{r}) = 4\int 
    \frac{T_{\mu\nu}(t-\left\lvert\vec{r}-\vec{r}'\right\rvert,\vec{r}')}{\left\lvert\vec{r}-\vec{r}'\right\rvert}\,\d V'.
\end{equation}
\begin{align}
    \hat{\bar{h}}_{\mu\nu}(\omega,\vec{r})&:=\frac{1}{\sqrt{2\pi}}
    \int\bar{h}_{\mu\nu}(t,\vec{r})e^{i\omega t}\d t\\
    &=4\int 
    \frac{\hat{T}_{\mu\nu}(\omega,\vec{r}')}{\left\lvert\vec{r}-\vec{r}'\right\rvert}e^{i\omega\left\lvert\vec{r}-\vec{r}'\right\rvert}\,\d V'.
\end{align}
由$\p^{\nu}\bar{h}_{\mu\nu}=0$,
\begin{equation}
    -i\omega\hat{\bar{h}}_{0\mu}=\sum_{i}\frac{\p\hat{\bar{h}}_{i\mu}}{\p x^{i}}.
\end{equation}
$\left\lvert \vec{r}\right\rvert \gg \left\lvert \vec{r}'\right\rvert$且$\omega\ll1/\left\lvert \vec{r}'\right\rvert$,
\begin{equation}
    \hat{\bar{h}}_{ij}(\omega,\vec{r}) = 4
    \frac{e^{i\omega\left\lvert\vec{r}\right\rvert}}{\left\lvert\vec{r}\right\rvert}
    \int \hat{T}_{ij}(\omega,\vec{r}')\,\d V'.
\end{equation}
\begin{align}
    \int \hat{T}_{ij}\,\d V'
    &=\int \sum_{k}(\hat{T}_{kj}\frac{\p x'^i}{\p x'^k})\,\d V'\\
    &= \sum_{k}\left[\int \frac{\p }{\p x'^k}(\hat{T}_{kj}x'^i)\,\d V'-\int \frac{\p \hat{T}_{kj}}{\p x'^k}x'^i\,\d V'\right]\\
    &= \sum_{k}\int \p'_k\,(\hat{T}_{kj}x'^i)\,\d V' - \sum_{k}\int \frac{\p \hat{T}_{kj}}{\p x'^k}x'^i\,\d V'\\
    &= \int \hat{T}_{kj}x'^i\,\d S' - \sum_{k}\int \frac{\p \hat{T}_{kj}}{\p x'^k}x'^i\,\d V'\\
    &= -\sum_{k}\int \frac{\p \hat{T}_{kj}}{\p x'^k}x'^i\,\d V'\\
    &= -\int (\sum_{k}\p'_k\hat{T}_{kj})x'^i\,\d V'\\
    &= -\int (\p_0\hat{T}_{0j})x'^i\,\d V'\\
    &= -i\omega\int \hat{T}_{0j}x'^i\,\d V'\\
    &= \int \hat{T}_{(ij)}\,\d V'\\
    &= -i\omega\int \hat{T}_{0(j}x'^{i)}\,\d V'\\
    &= -\frac{i\omega}{2}\int (\hat{T}_{0j}x'^{i}+\hat{T}_{0i}x'^{j})\,\d V',\\
\end{align}
\begin{align}
    -\frac{i\omega}{2}\int (\hat{T}_{0j}x'^{i}+\hat{T}_{0i}x'^{j})\,\d V'
    &= -\frac{i\omega}{2}\int \sum_{k}(\hat{T}_{0k}x'^{i}\frac{\p x'^{j}}{\p x'^{k}}+\hat{T}_{0k}\frac{\p x'^{i}}{\p x'^{k}}x'^{j})\,\d V'\\
    &= -\frac{i\omega}{2}\sum_{k}\left[\int \frac{\p }{\p x'^k}(\hat{T}_{0k}x'^ix'^j)\,\d V'-\int \frac{\p \hat{T}_{0k}}{\p x'^k}x'^ix'^j\,\d V'\right]\\
    &= -\frac{i\omega}{2}\sum_{k}\int \p'_k\,(\hat{T}_{0k}x'^ix'^j)\,\d V' +\frac{i\omega}{2}\sum_{k}\int \frac{\p \hat{T}_{0k}}{\p x'^k}x'^ix'^j\,\d V'\\
    &= -\frac{i\omega}{2}\sum_{k}\int \hat{T}_{0k}x'^ix'^j\,\d S' +\frac{i\omega}{2}\sum_{k}\int \frac{\p \hat{T}_{0k}}{\p x'^k}x'^ix'^j\,\d V'\\
    &= \frac{i\omega}{2}\sum_{k}\int \frac{\p \hat{T}_{0k}}{\p x'^k}x'^ix'^j\,\d V'\\
    &= \frac{i\omega}{2}\int (\sum_{k}\p'_k\hat{T}_{0k})x'^ix'^j\,\d V'\\
    &= \frac{i\omega}{2}\int (\p_0\hat{T}_{00})x'^ix'^j\,\d V'\\
    &= -\frac{\omega^2}{2}\int \hat{T}_{00}\,x'^ix'^j\,\d V'.
\end{align}
\begin{equation}
    q_{ij}(t):=\int{T}_{00}\,x'^ix'^j\,\d V',
\end{equation}
\begin{equation}
    \hat{\bar{h}}_{ij}(\omega,\vec{r}) = -2\omega^2\frac{e^{i\omega\left\lvert\vec{r}\right\rvert}}{\left\lvert\vec{r}\right\rvert}\hat{q}_{ij}(\omega),
\end{equation}
\begin{equation}
    {\bar{h}}_{ij}(t,\vec{r}) = \frac{2}{\left\lvert\vec{r}\right\rvert}
    \frac{\d^2}{\d t^2}{q}_{ij}(t-\left\lvert\vec{r}\right\rvert).\label{qf}
\end{equation}

\section{$+$ Mode and $\times$ Mode}

寻新标架$(e'^1)_a=(e^+)_a$, $(e'^2)_a=(e^\times)_a$, $(e'^3)_a=(e^r)_a$, ${\bar{h}}_{ij}(e^i)_a(e^j)_b={\bar{h}}'_{ij}(e'^i)_a(e'^j)_b$, 取$x$, $y$分量后去迹, $h_+=\frac{1}{2}({\bar{h}}'_{11}-{\bar{h}}'_{22})$, $h_\times={\bar{h}}'_{12}={\bar{h}}'_{21}$? \cite{Sathyaprakash2009}

\cite{Blanchet1997}, $\vec{n}:=\frac{\vec{r}}{\left\lvert\vec{r}\right\rvert}$,
\begin{equation}
    h_{ij}^{\text{TT}}=\frac{2}{\left\lvert\vec{r}\right\rvert}\mathcal{P}_{ijkm}\frac{\d^2}{\d t^2}{Q}^{km}(t-\left\lvert\vec{r}\right\rvert), \label{TT}
\end{equation}
\begin{equation}
    \mathcal{P}_{ijkm}:=
    \left(\delta_{ik} -\vec{n}_i\vec{n}_k\right)
    \left(\delta_{jm} -\vec{n}_j\vec{n}_m\right)
    -\frac{1}{2}
    \left(\delta_{ij} -\vec{n}_i\vec{n}_j\right)
    \left(\delta_{km} -\vec{n}_k\vec{n}_m\right),
\end{equation}
\begin{equation}
    Q^{km}(t):=\int{T}_{00}\,\left(x'^kx'^m-\frac{1}{3}\delta^{km}\sum_nx'^nx'^n\right)\,\d V'
\end{equation}

\section{电磁---引力对比}

\begin{equation}
    A_\mu(t,\vec{r})=\frac{\mu_0}{4\pi}\int\frac{J_\mu(t-\left\lvert \vec{r}-\vec{r}'\right\rvert ,\vec{r}')}{\left\lvert \vec{r}-\vec{r}'\right\rvert}\d V'
\end{equation}
\begin{equation}
    \bar{h}_{\mu\nu}(t,\vec{r})=4G\int\frac{T_{\mu\nu}(t-\left\lvert\vec{r}-\vec{r}'\right\rvert,\vec{r}')}{\left\lvert\vec{r}-\vec{r}'\right\rvert}\,\d V'
\end{equation}

\begin{equation}
    A_\mu(t,\vec{r})=\frac{1}{\sqrt{2\pi}}
    \int\hat{A}_{\mu}(\omega,\vec{r})e^{-i\omega t}\d t
\end{equation}
\begin{equation}
    \bar{h}_{\mu\nu}(t,\vec{r})=\frac{1}{\sqrt{2\pi}}
    \int\hat{\bar{h}}_{\mu\nu}(\omega,\vec{r})e^{-i\omega t}\d t
\end{equation}

\begin{equation}
    \hat{A}_{\mu}(\omega,\vec{r})=\frac{\mu_0}{4\pi}\int\frac{\hat{J}_{\mu}(\omega,\vec{r}')}{\left\lvert\vec{r}-\vec{r}'\right\rvert}e^{i\omega\left\lvert\vec{r}-\vec{r}'\right\rvert}\,\d V'
\end{equation}
\begin{equation}
    \hat{\bar{h}}_{\mu\nu}(\omega,\vec{r})=4G\int\frac{\hat{T}_{\mu\nu}(\omega,\vec{r}')}{\left\lvert\vec{r}-\vec{r}'\right\rvert}e^{i\omega\left\lvert\vec{r}-\vec{r}'\right\rvert}\,\d V'
\end{equation}

\begin{equation}
    \hat{A}_{\mu}(\omega,\vec{r})=\frac{\mu_0}{4\pi}\frac{e^{i\omega\left\lvert\vec{r}\right\rvert}}{\left\lvert\vec{r}\right\rvert}\int\hat{J}_{\mu}(\omega,\vec{r}')e^{-i\omega(\frac{\vec{r}}{\left\lvert\vec{r}\right\rvert}\cdot\vec{r}')}\,\d V'
\end{equation}
\begin{equation}
    \hat{\bar{h}}_{\mu\nu}(\omega,\vec{r})=4G\frac{e^{i\omega\left\lvert\vec{r}\right\rvert}}{\left\lvert\vec{r}\right\rvert}\int\hat{T}_{\mu\nu}(\omega,\vec{r}')e^{-i\omega(\frac{\vec{r}}{\left\lvert\vec{r}\right\rvert}\cdot\vec{r}')}\,\d V'
\end{equation}

\begin{equation}
    \hat{A}_{\mu}(\omega,\vec{r})=\frac{\mu_0}{4\pi}\frac{e^{i\omega\left\lvert\vec{r}\right\rvert}}{\left\lvert\vec{r}\right\rvert}\int\hat{J}_{\mu}(\omega,\vec{r}')\left[1-i\omega(\frac{\vec{r}}{\left\lvert\vec{r}\right\rvert}\cdot\vec{r}')-\dots\right]\,\d V'
\end{equation}
\begin{equation}
    \hat{\bar{h}}_{\mu\nu}(\omega,\vec{r})=4G\frac{e^{i\omega\left\lvert\vec{r}\right\rvert}}{\left\lvert\vec{r}\right\rvert}\int\hat{T}_{\mu\nu}(\omega,\vec{r}')\left[1-i\omega(\frac{\vec{r}}{\left\lvert\vec{r}\right\rvert}\cdot\vec{r}')-\dots\right]\,\d V'
\end{equation}

\subsection{电偶极---引力对比}

\begin{equation}
    \hat{A}_i=\frac{\mu_0}{4\pi}\frac{e^{i\omega\left\lvert\vec{r}\right\rvert}}{\left\lvert\vec{r}\right\rvert}\int\hat{J}_i\,\d V'
\end{equation}
\begin{equation}
    \hat{\bar{h}}_{ij}=4G\frac{e^{i\omega\left\lvert\vec{r}\right\rvert}}{\left\lvert\vec{r}\right\rvert}\int\hat{T}_{ij}\,\d V'
\end{equation}

\begin{equation}
    \int \hat{J}_{i}\,\d V'=-i\omega\int\hat{J}_{0}x'^i\,\d V'
\end{equation}
\begin{equation}
    \int\hat{T}_{ij}\,\d V'=-\frac{\omega^2}{2}\int \hat{T}_{00}\,x'^ix'^j\,\d V'
\end{equation}

\begin{equation}
    \hat{p}_i=\int\hat{J}_{0}x'^i\,\d V'
\end{equation}
\begin{equation}
    \hat{q}_{ij}=\int \hat{T}_{00}\,x'^ix'^j\,\d V'
\end{equation}

\begin{equation}
    \hat{A}_i=\frac{\mu_0}{4\pi}\frac{e^{i\omega\left\lvert\vec{r}\right\rvert}}{\left\lvert\vec{r}\right\rvert}(-i\omega \hat{p}_i)
\end{equation}
\begin{equation}
    \hat{\bar{h}}_{ij}=4G\frac{e^{i\omega\left\lvert\vec{r}\right\rvert}}{\left\lvert\vec{r}\right\rvert}(-\frac{\omega^2}{2}\hat{q}_{ij})
\end{equation}

\begin{equation}
    {A}_i=\frac{\mu_0}{4\pi}\frac{1}{\left\lvert\vec{r}\right\rvert}\frac{\d}{\d t}p_i(t-\left\lvert\vec{r}\right\rvert)
\end{equation}
\begin{equation}
    {\bar{h}}_{ij}=4G\frac{1}{\left\lvert\vec{r}\right\rvert}\frac{1}{2}\frac{\d^2}{\d t^2}q_{ij}(t-\left\lvert\vec{r}\right\rvert)
\end{equation}

\subsection{电四极---引力对比}

\begin{equation}
    \hat{A}_{i}(\omega,\vec{r})=\frac{\mu_0}{4\pi}\frac{e^{i\omega\left\lvert\vec{r}\right\rvert}}{\left\lvert\vec{r}\right\rvert}（）(-i\omega)\int\hat{J}_{i}(\omega,\vec{r}')(\frac{\vec{r}}{\left\lvert\vec{r}\right\rvert}\cdot\vec{r}')\,\d V'
\end{equation}

\begin{equation}
    \hat{A}_i=\frac{\mu_0}{4\pi}\frac{e^{i\omega\left\lvert\vec{r}\right\rvert}}{\left\lvert\vec{r}\right\rvert}(-i\omega)\int\hat{J}_i'n^j{x}_j'\,\d V'
\end{equation}

\begin{equation}
    \hat{A}_i=\frac{\mu_0}{4\pi}\frac{e^{i\omega\left\lvert\vec{r}\right\rvert}}{\left\lvert\vec{r}\right\rvert}(-i\omega)\int n^j{x}_j'\hat{J}_i'\,\d V'
\end{equation}

\begin{equation}
    \hat{A}_i=\frac{\mu_0}{4\pi}\frac{e^{i\omega\left\lvert\vec{r}\right\rvert}}{\left\lvert\vec{r}\right\rvert}(-i\omega)n^j\!\left[\int {x}_{(j}'\hat{J}_{i)}'\,\d V'\right]
\end{equation}

\begin{align}
    \int {x}_{(j}'\hat{J}_{i)}'\,\d V'
    &= \frac{1}{2}\int (\hat{J}_{j}'{x}_{i}'+\hat{J}_{i}'{x}_{j}')\,\d V'\\
    &= \frac{1}{2}\int \sum_{k}(\hat{J}_{k}'x'^{i}\frac{\p x'^{j}}{\p x'^{k}}+\hat{J}_{k}'\frac{\p x'^{i}}{\p x'^{k}}x'^{j})\,\d V'\\
    &= \frac{1}{2}\sum_{k}\left[\int \frac{\p }{\p x'^k}(\hat{J}_{k}'x'^ix'^j)\,\d V'-\int \frac{\p \hat{J}_{k}'}{\p x'^k}x'^ix'^j\,\d V'\right]\\
    &= \frac{1}{2}\sum_{k}\int \p'_k\,(\hat{J}_{k}'x'^ix'^j)\,\d V' -\frac{1}{2}\sum_{k}\int \frac{\p \hat{J}_{k}'}{\p x'^k}x'^ix'^j\,\d V'\\
    &= \frac{1}{2}\sum_{k}\int \hat{J}_{k}'x'^ix'^j\,\d S' -\frac{1}{2}\sum_{k}\int \frac{\p \hat{J}_{k}'}{\p x'^k}x'^ix'^j\,\d V'\\
    &= -\frac{1}{2}\sum_{k}\int \frac{\p \hat{J}_{k}'}{\p x'^k}x'^ix'^j\,\d V'\\
    &= -\frac{1}{2}\int (\sum_{k}\p'_k\hat{J}_{k}')x'^ix'^j\,\d V'\\
    &= -\frac{1}{2}\int (\p_0\hat{J}_{0}')x'^ix'^j\,\d V'\\
    &= -\frac{i\omega}{2}\int \hat{J}_{0}'x'^ix'^j\,\d V'
\end{align}

\begin{equation}
    \hat{D}_{ij}=\int \hat{J}_{0}'\,x'^ix'^j\,\d V'
\end{equation}

\begin{equation}
    \hat{A}_i=\frac{\mu_0}{4\pi}\frac{e^{i\omega\left\lvert\vec{r}\right\rvert}}{\left\lvert\vec{r}\right\rvert}(-\frac{\omega^2}{2}n^j\hat{D}_{ij}
    )
\end{equation}

\begin{equation}
    {A}_i=\frac{\mu_0}{4\pi}\frac{1}{\left\lvert\vec{r}\right\rvert}n^j\frac{1}{2}\frac{\d^2}{\d t^2}D_{ij}(t-\left\lvert\vec{r}\right\rvert)
\end{equation}

\section{Varying $G$}

\begin{equation}
    T_{ab}=2U_{(a}J_{b)}+U^cJ_cU_aU_b
\end{equation}
\begin{equation}
    J_b=-U^aT_{ab}
\end{equation}
\begin{equation}
    \p^a\bar{h}_{ab}=0
\end{equation}
\begin{equation}
    \p^c\p_c\bar{h}_{ab}=-16\pi\frac{G_0}{c_0^3}T_{ab}
\end{equation}
\begin{equation}
    \Gamma^c_{\ph{c}ab}=\frac{1}{2}\eta^{cd}(2\p_{(a}{h}_{b)d}-\p_d{h}_{ab})
\end{equation}
\begin{equation}
    U^a\p_aU^c+\Gamma^c_{\ph{c}ab}U^aU^b=0
\end{equation}
\begin{equation}
    U^a\p_aU^c=-\frac{1}{2}\eta^{cd}(2\p_{(a}{h}_{b)d}-\p_d{h}_{ab})U^aU^b
\end{equation}

\begin{equation}
    A_b
    =-\frac{1}{4}U^a\bar{h}_{ab}
\end{equation}
\begin{equation}
    A_0
    =-\frac{1}{4}c_0\bar{h}_{00}
    =-\frac{1}{2}c_0(\bar{h}_{00}-\frac{1}{2}\eta_{00}\eta^{00}\bar{h}_{00})=-\frac{1}{2}c_0h_{00}
\end{equation}
\begin{equation}
    A_i=-\frac{1}{4}c_0\bar{h}_{0i}=-\frac{1}{4}c_0{h}_{0i}
\end{equation}

\begin{equation}
    U^\mu\p_\mu U^i=-\frac{1}{2}\eta^{i\sigma}(\p_\mu{h}_{\nu\sigma}+\p_\nu{h}_{\mu\sigma}-\p_\sigma{h}_{\mu\nu})U^\mu U^\nu
\end{equation}
\begin{align}
    -\frac{1}{2}\eta^{i\sigma}(\p_0{h}_{0\sigma}+\p_0{h}_{0\sigma}-\p_\sigma{h}_{00})U^0 U^0
    &=\frac{1}{2}c_0^2\eta^{i\sigma}\p_\sigma{h}_{00}\\
    &=\frac{1}{2}c_0^2\p^i{h}_{00}\\
    &=c_0\p^iA_0\\
    &=-E^i
\end{align}
\begin{align}
    -\frac{1}{2}\eta^{i\sigma}(\p_0{h}_{j\sigma}+\p_j{h}_{0\sigma}-\p_\sigma{h}_{0j})U^0 U^j
    &=-\frac{1}{2}c_0\eta^{i\sigma}(\p_j{h}_{0\sigma}-\p_\sigma{h}_{0j})v^j\\
    &=-\frac{1}{2}c_0\eta^{ik}(\p_j{h}_{0k}-\p_k{h}_{0j})v^j\\
    &=2\eta^{ik}(\p_jA_k-\p_kA_j)v^j\\
    &=2(\p_jA^i-\p^iA_j)v^j\\
    &=-2\varepsilon^{i}_{\ph{i}jk}v^jB^k
\end{align}
\begin{align}
    -\frac{1}{2}\eta^{i\sigma}(\p_j{h}_{k\sigma}+\p_k{h}_{j\sigma}-\p_\sigma{h}_{jk})U^j U^k=0
\end{align}
\begin{equation}
    a^i=-E^i-4\varepsilon^{i}_{\ph{i}jk}v^jB^k
\end{equation}

\begin{equation}
    \p^i(\frac{c_0}{16\pi G_0}E_i)=\rho
\end{equation}
\begin{equation}
    \p^iB_i=0
\end{equation}
\begin{equation}
    \varepsilon^{i}_{\ph{i}jk}\p^jE^k=-\p_tB^i
\end{equation}
\begin{equation}
    \varepsilon^{i}_{\ph{i}jk}\p^j(\frac{c_0^3}{16\pi G_0}B^k)=j^i+\p_t(\frac{c_0}{16\pi G_0}E^i)
\end{equation}

\begin{equation}
    \p^{\nu}\p_{\nu}A_{\mu}=-\mu J_{\mu},\quad
    \p^{\mu}A_{\mu}=0
\end{equation}
\begin{equation}
    \vec{\nabla}^2\varphi-\frac{\p^2}{\p t^2}\varphi=-\mu\rho
\end{equation}
\begin{equation}
    \vec{\nabla}^2\vec{A}-\frac{\p^2}{\p t^2}\vec{A}=-\mu\vec{j}
\end{equation}
\begin{equation}
    \frac{\p}{\p t}\varphi+\vec{\nabla}\cdot\vec{A}=0
\end{equation}
\begin{equation}
    \varphi_1=\varphi_2
\end{equation}
\begin{equation}
    \vec{A}_1=\vec{A}_2
\end{equation}
\begin{equation}
    \frac{1}{\mu_1}\vec{n}\cdot(\vec{\nabla}\varphi_1+\frac{\p}{\p t}\vec{A}_1)=\frac{1}{\mu_2}\vec{n}\cdot(\vec{\nabla}\varphi_2+\frac{\p}{\p t}\vec{A}_2)
\end{equation}
\begin{equation}
    \frac{1}{\mu_1}\vec{n}\times(\vec{\nabla}\times\vec{A}_1)=\frac{1}{\mu_2}\vec{n}\times(\vec{\nabla}\times\vec{A}_2)
\end{equation}
\begin{equation}
    \frac{1}{\mu_1}[(\vec{n}\cdot\vec{\nabla})\varphi_1+\frac{\p}{\p t}(\vec{n}\cdot\vec{A}_1)]=\frac{1}{\mu_2}[(\vec{n}\cdot\vec{\nabla})\varphi_2+\frac{\p}{\p t}(\vec{n}\cdot\vec{A}_2)]
\end{equation}
\begin{equation}
    \frac{1}{\mu_1}[(\vec{n}\cdot\vec{\nabla})\vec{A}_1-\vec{\nabla}(\vec{n}\cdot\vec{A}_1)]=\frac{1}{\mu_2}[(\vec{n}\cdot\vec{\nabla})\vec{A}_2-\vec{\nabla}(\vec{n}\cdot\vec{A}_2)]
\end{equation}
\begin{equation}
    \varphi=\varphi_0e^{i(\omega t-\vec{k}\cdot\vec{r})}
\end{equation}
\begin{equation}
    \vec{A}=\vec{A}_0e^{i(\omega t-\vec{k}\cdot\vec{r})}
\end{equation}
\begin{equation}
    \varphi=\varphi e^{i(\omega t-\vec{k}\cdot\vec{r})}+\varphi' e^{i(\omega t+\vec{k}\cdot\vec{r})}
\end{equation}
\begin{equation}
    \vec{A}=\vec{A} e^{i(\omega t-\vec{k}\cdot\vec{r})}+\vec{A}' e^{i(\omega t+\vec{k}\cdot\vec{r})}
\end{equation}
\begin{equation}
    \varphi=\varphi''e^{i(\omega t-\vec{k}\cdot\vec{r})}
\end{equation}
\begin{equation}
    \vec{A}=\vec{A}''e^{i(\omega t-\vec{k}\cdot\vec{r})}
\end{equation}
\begin{equation}
    \omega(\varphi+\varphi')=-\vec{k}\cdot(\vec{A}-\vec{A}')
\end{equation}
\begin{equation}
    \omega\varphi''=-\vec{k}\cdot\vec{A}''
\end{equation}
\begin{equation}
    \varphi+\varphi'=\varphi''
\end{equation}
\begin{equation}
    \vec{A}+\vec{A}'=\vec{A}''
\end{equation}
\begin{equation}
    \frac{1}{\mu_1}[-(\vec{n}\cdot\vec{k})(\varphi-\varphi')+\omega(\vec{n}\cdot(\vec{A}+\vec{A}'))]=\frac{1}{\mu_2}[-(\vec{n}\cdot\vec{k})\varphi''+\omega(\vec{n}\cdot\vec{A}'')]
\end{equation}
\begin{equation}
    \frac{1}{\mu_1}[-(\vec{n}\cdot\vec{k})(\vec{A}-\vec{A}')+\vec{k}(\vec{n}\cdot(\vec{A}-\vec{A}'))]=\frac{1}{\mu_2}[-(\vec{n}\cdot\vec{k})\vec{A}''+\vec{k}(\vec{n}\cdot\vec{A}'')]
\end{equation}
\begin{equation}
    \omega(\varphi+\varphi')=-\omega\vec{n}\cdot(\vec{A}-\vec{A}')
\end{equation}
\begin{equation}
    \omega\varphi''=-\omega\vec{n}\cdot\vec{A}''
\end{equation}
\begin{equation}
    (\varphi+\varphi')=\varphi''
\end{equation}
\begin{equation}
    (\vec{A}+\vec{A}')=\vec{A}''
\end{equation}
\begin{equation}
    \frac{1}{\mu_1}[-\omega(\varphi-\varphi')+\omega(\vec{n}\cdot(\vec{A}+\vec{A}'))]=\frac{1}{\mu_2}[-\omega\varphi''+\omega(\vec{n}\cdot\vec{A}'')]
\end{equation}
\begin{equation}
    \frac{1}{\mu_1}[-\omega(\vec{A}-\vec{A}')+\omega\vec{n}(\vec{n}\cdot(\vec{A}-\vec{A}'))]=\frac{1}{\mu_2}[-\omega\vec{A}''+\omega\vec{n}(\vec{n}\cdot\vec{A}'')]
\end{equation}
\begin{equation}
    (\varphi+\varphi')=-(\vec{A}_\text{n}-\vec{A}'_\text{n})
\end{equation}
\begin{equation}
    \varphi''=-\vec{A}''_\text{n}
\end{equation}
\begin{equation}
    (\varphi+\varphi')=\varphi''
\end{equation}
\begin{equation}
    (\vec{A}_\text{n}+\vec{A}'_\text{n})=\vec{A}''_\text{n}
\end{equation}
\begin{equation}
    (\vec{A}_\text{t}+\vec{A}'_\text{t})=\vec{A}''_\text{t}
\end{equation}
\begin{equation}
    \frac{1}{\mu_1}[-(\varphi-\varphi')+(\vec{A}_\text{n}+\vec{A}'_\text{n})]=\frac{1}{\mu_2}[-\varphi''+\vec{A}''_\text{n}]
\end{equation}
\begin{equation}
    \frac{1}{\mu_1}[(\vec{A}_\text{t}-\vec{A}'_\text{t})]=\frac{1}{\mu_2}[\vec{A}''_\text{t}]
\end{equation}
\begin{equation}
    \varphi'=\frac{\mu_2-\mu_1}{\mu_1}\varphi,\quad\vec{A}'_\text{n}=0\vec{A}_\text{n}
\end{equation}
\begin{equation}
    \varphi''=\frac{\mu_2}{\mu_1}\varphi,\quad\vec{A}''_\text{n}=1\vec{A}_\text{n}
\end{equation}
\begin{equation}
    (\varphi'+\vec{A}'_\text{n})=-\frac{\mu_2-\mu_1}{\mu_2+\mu_1}(-\varphi+\vec{A}_\text{n})
\end{equation}
\begin{equation}
    (-\varphi''+\vec{A}''_\text{n})=\frac{2\mu_2}{\mu_2+\mu_1}(-\varphi+\vec{A}_\text{n})
\end{equation}
\begin{equation}
    \vec{A}'_\text{t}=\frac{\mu_2-\mu_1}{\mu_2+\mu_1}\vec{A}_\text{t}
\end{equation}
\begin{equation}
    \vec{A}''_\text{t}=\frac{2\mu_2}{\mu_2+\mu_1}\vec{A}_\text{t}
\end{equation}
\begin{equation}
    \vec{S}'=-\frac{(\mu_1-\mu_2)^2}{(\mu_1+\mu_2)^2}\vec{S}
\end{equation}
\begin{equation}
    \vec{S}''=\frac{4\mu_1\mu_2}{(\mu_1+\mu_2)^2}\vec{S}
\end{equation}
\begin{equation}
    \Delta r
\end{equation}
\begin{equation}
    \mu_1,\dots,\mu_n
\end{equation}
\begin{equation}
    1+\frac{\mu_2-\mu_1}{\mu_2+\mu_1},\dots,1+\frac{\mu_n-\mu_{n-1}}{\mu_n+\mu_{n-1}}
\end{equation}
\begin{equation}
    \frac{\mu_1}{\mu_2}(1+\frac{\mu_2-\mu_1}{\mu_2+\mu_1})^2,\dots,\frac{\mu_{n-1}}{\mu_n}(1+\frac{\mu_n-\mu_{n-1}}{\mu_n+\mu_{n-1}})^2
\end{equation}
\begin{equation}
    \prod_{i=1}^{n-1}(1+\frac{\mu_{i+1}-\mu_i}{\mu_{i+1}+\mu_i})
\end{equation}
\begin{equation}
    \sum_{i=1}^{n-1}\ln(1+\frac{\mu_{i+1}-\mu_i}{\mu_{i+1}+\mu_i})
\end{equation}
\begin{equation}
    \sum_{i=1}^{n-1}((\frac{\mu_{i+1}-\mu_i}{\mu_{i+1}+\mu_i})-\frac{1}{2}(\frac{\mu_{i+1}-\mu_i}{\mu_{i+1}+\mu_i})^2+\frac{1}{3}(\frac{\mu_{i+1}-\mu_i}{\mu_{i+1}+\mu_i})^3-\dots)
\end{equation}
\begin{equation}
    \sum_{i=1}^{n-1}(\frac{\mu_{i+1}-\mu_i}{\mu_{i+1}+\mu_i})
\end{equation}
\begin{equation}
    \int\frac{1}{2\mu}\frac{\d u}{\d r}\d r
\end{equation}
\begin{equation}
    \frac{1}{2}\Delta\ln\mu
\end{equation}
\begin{equation}
    \sqrt{\frac{\mu_n}{\mu_1}}
\end{equation}
\begin{equation}
    1
\end{equation}
