\chapter{宇宙学效应}

\section{Luminosity Distance}

\cite{Maggiore2014},
\begin{equation}
    \int_{t_\t{emis}}^{t_\t{obs}}\frac{c\,\d t}{a(t)}=    \int_{t_\t{emis}+\Delta t_\t{emis}}^{t_\t{obs}+\Delta t_\t{obs}}\frac{c\,\d t}{a(t)}=\int_0^r\frac{\d r}{(1-kr^2)^{1/2}},
\end{equation}
故$\Delta t_\t{obs}=\Delta t_\t{emis}(1+z)$. 另由$E=\hbar\omega$, 有$\Delta E_\t{obs}=\Delta E_\t{emis}(1+z)$, 故$d_\t{L}=a(t_\t{obs})r(1+z)$.

不用光子论, 见\cite{Ellis2012} 7.4 节.

\section{Propagation}

\begin{equation}
    \d s^2=-\d t^2+a^2[\frac{\d r^2}{1-kr^2}+r^2(\d\theta^2+\sin^2\theta\,\d\phi^2)],
\end{equation}
$\d t:=a\d\eta$, $(1/\sqrt{1-kr^2})\d r:=\d\psi$,
\begin{equation}
    \d s^2=a^2[-\d\eta^2+\d\psi^2+r(\psi)^2(\d\theta^2+\sin^2\theta\,\d\phi^2)].
\end{equation}
\cite{Maggiore2014}, $\square\Phi(\eta,\psi):=0$, %$\Phi:=f/r$, $f:=g/a$,
\begin{comment}
\begin{equation}
    \sqrt{-g}=a^4r^2\sin\theta,
\end{equation}
\begin{equation}
    \p_\eta(-(a^4r^2\sin\theta)a^{-2}\p_\eta\Phi)+\p_\psi((a^4r^2\sin\theta)a^{-2}\p_\psi\Phi)=0,
\end{equation}
\end{comment}
\begin{equation}
    -\p_\eta(a^2r^2\p_\eta\Phi)+\p_\psi(a^2r^2\p_\psi\Phi)=0,
\end{equation}
\begin{equation}
    - a r \frac{\partial^{2}\Phi}{\partial \eta^{2}}  + a r \frac{\partial^{2}\Phi}{\partial \psi^{2}}  + 2 a \frac{\partial\Phi}{\partial \psi}  \frac{\d r}{\d \psi}  - 2 r \frac{\partial\Phi}{\partial \eta}  \frac{\d a}{\d \eta} =0,
\end{equation}
$\Phi:=g/ar$,
\begin{equation}
    - a g \frac{\d^{2}r}{\d \psi^{2}}  - a r \frac{\partial^{2}g}{\partial \eta^{2}}  + a r \frac{\partial^{2}g}{\partial \psi^{2}}  + g r \frac{\d^{2}a}{\d \eta^{2}} =0.
\end{equation}
${\d^{2}r/\d \psi^{2}}=kr$,
\begin{equation}
    \p_\psi^2g-kg+(\p_\eta^2a/a)g-\p_\eta^2g=0,
\end{equation}
$\p_\eta^2a/a\sim\eta^2$, 故$k = 0$时, 若$\omega^2\gg1/\eta^2$,
\begin{equation}
    g\simeq e^{i\omega(\eta-\psi)}=e^{i\omega(\eta-r)}.
\end{equation}
$g:=N(\eta)\varPsi(\psi)$,
\begin{equation}
    N\p_\psi^2\varPsi-kN\varPsi-\varPsi\p_\eta^2N\simeq0,
\end{equation}
\begin{equation}
    \varPsi^{-1}\p_\psi^2\varPsi-k\simeq N^{-1}\p_\eta^2N:\simeq C,
\end{equation}
\begin{equation}
    \varPsi\simeq e^{\sqrt{k-C}\psi},
\end{equation}
\begin{equation}
    N\simeq e^{\sqrt{-C}\eta},
\end{equation}
\begin{equation}
    g\simeq e^{i(\omega\eta-\sqrt{\omega^2-k}\psi)}.
\end{equation}
